\documentclass[a4paper, 10pt, fleqn, twocolumn, twoside]{article}
\usepackage[utf8]{inputenc}
\usepackage{ngerman}
\usepackage{parskip}
\usepackage{geometry}
\usepackage{amsmath,amssymb}
\usepackage{color}
\definecolor{c1}{rgb}{0.4,0.0,0.2}
\usepackage[colorlinks=true,linkcolor=c1]{hyperref}
\geometry{a4paper,left=20mm,right=20mm, top=20mm, bottom=10mm}
% Keine Seitenanzahl:
\pagestyle{empty}
\newcommand{\ds}{\displaystyle}
\newcommand{\nb}{\nopagebreak}
\newcommand{\hbf}[1]{\textbf{#1}\nopagebreak}

\setlength{\columnsep}{6mm}

\begin{document}

$\sin(a+b) = \sin a\cos b + \sin b\cos a$\\
$\cos(a+b) = \cos a\cos b - \sin a\sin b$\\
${}\!\!\!\begin{array}{l|l}
\sin(-x) = -\sin x & \sin(\pi/2-x)=\cos x\\
\cos(-x) = \cos x & \cos(\pi/2-x)=\sin x
\end{array}$\\
${}\!\!\!\begin{array}{l|l}
\sin^2 x+\cos^2 x=1
& 2i\sin x = e^{ix}-e^{-ix}\\
e^{ix} = \cos x+i\sin x
& 2\cos x = e^{ix}+e^{-ix}
\end{array}$\\
${}\!\!\!\begin{array}{l|l}
\cosh^2 x-\sinh^2 x=1
& 2\sinh x = e^x-e^{-x}\\
e^{x} = \cosh x+\sinh x
& 2\cosh x = e^x+e^{-x}
\end{array}$\\
$\cos(2x) = 1-2\sin^2 x = 2\cos^2 x-1$\\
$\sin(nx) = 2\cos x \sin((n-1)x)-\sin((n-2)x)$\\
$\cos(nx) = 2\cos x \cos((n-1)x)-\cos((n-2)x)$\\
$s_n = a_1+\ldots+a_n$\\
${}\!\!\!\begin{array}{l|l}
a_k=k & s_n=(n/2)(n+1)\\
a_k=k^2 & s_n=(n/6)(n+1)(2n+1)\\
a_k=k^3 & s_n=(n/2)^2(n+1)^2
\end{array}$\\
$\ds\sum_{k=a}^{b-1} q^k = \frac{q^b-q^a}{q-1},\quad
\sum_{k=a}^{b-1} k^m q^k
= \Big(q\frac{\mathrm d}{\mathrm dq}\Big)^m
\,\frac{q^b-q^a}{q-1}$\\
$\ds e^x = \sum_{k=0}^{\infty} \frac{x^k}{k!},\quad
\frac{x}{e^x-1} = \sum_{k=0}^{\infty} \overline{B}_k\frac{x^k}{k!},\quad
\frac{1}{1-x} = \sum_{k=0}^\infty x^k$\\
$\ds e^x = \lim_{n\rightarrow\infty} \Big(1+\frac{x}{n}\Big)^n,
\quad\ln x = \lim_{h\rightarrow 0}\frac{x^h-1}{h}$\\
$\ds \ln(1-x) = (-1)\sum_{k=1}^{\infty} \frac{x^k}{k}
\quad (-1\le x<1)$\\
${}\!\!\!\begin{array}{l|l}
\ds\sin x = \sum_{k=0}^{\infty}
(-1)^k \frac{x^{2k+1}}{(2k+1)!}
& \ds\sinh x = \sum_{k=0}^{\infty}\frac{x^{2k+1}}{(2k+1)!}\\
\ds\cos x = \sum_{k=0}^{\infty}
(-1)^k \frac{x^{2k}}{(2k)!}
& \ds\cosh x = \sum_{k=0}^{\infty}\frac{x^{2k}}{(2k)!}
\end{array}$\\
$\ds (x+1)^n = \sum_{k=0}^{\infty} \binom{n}{k} x^k\quad (|x|<1)$\\
$\ds\frac{1}{(1-x)^n} = \sum_{k=0}^{\infty} \binom{n+k-1}{k} x^k
\quad (|x|<1)$

$x_{n+1} = \varphi(x_n),\quad \varphi(x) = x-f(x)/f'(x)$

$\ds f(x+h) \stackrel{\mathrm{??}}= \sum_{k=0}^\infty
\frac{\langle h,\nabla\rangle^k}{k!} f(x)
= e^{\langle h,\nabla\rangle}f(x)$\\
$n! \approx\sqrt{2\pi n}\,(n/e)^n$\\
$\ds n!\approx\sqrt{2\pi n}\,n^n \exp\Big(\frac{1}{12n}-n\Big)$

${}\!\!\!\begin{array}{l|l}
\sin'x=\cos x
& (fg)'=f'g+g'f\\
\cos'x = -\sin x
& (f/g)' = (f'g-g'f)/g^2\\
\tan'x = 1+\tan^2 x
& (1/g)' = -g'/g^2\\
\cot'x = -1-\cot^2 x
& (f(g))'=f'(g)g'\\
\arcsin'x = 1/\sqrt{1-x^2}
& (e^x)'=e^x\\
\arccos'x = -1/\sqrt{1-x^2}
& \ln'x = 1/x\\
\arctan'x = 1/(x^2+1)
& (x^n)'=nx^{n-1}
\end{array}$

${}\!\!\!\begin{array}{l|l}
t = \tan(x/2) & \ds\sin x = \frac{2t}{1+t^2}\\
\ds\mathrm dx = \frac{2\,\mathrm dt}{1+t^2}
& \ds\cos x = \frac{1-t^2}{1+t^2}
\end{array}$

$f(x) = f(2a-x)$ (Achsensymmetrie)\\
$f(x) = 2b-f(2a-x)$ (Punktsymmetrie)

$p(x) = y_0+a_1(x-x_0)+a_2(x-x_0)(x-x_1)$\\
$\ds a_1 = \frac{y_1-y_0}{x_1-x_0},\quad
a_2 = \frac{1}{x_2-x_1}
\Big(\frac{y_2-y_0}{x_2-x_0}-a_1\Big)$

\newpage
$\ds\int_a^b f(x)\,\mathrm dx
= \lim_{n\rightarrow\infty}\sum_{k=1}^n
f\!\Big(a+k\frac{b-a}{n}\Big)\frac{b-a}{n}$\\
$\ds\int_a^b fg'\,\mathrm dx
= [fg]_a^b - \int_a^b f'g\,\mathrm dx$\\
$\ds\int_a^b f(g)g'\,\mathrm dx
= \int_{g(a)}^{g(b)} f(u)\,\mathrm du$\\
$\ds\frac{\mathrm d}{\mathrm dx}
\int_{a(x)}^{b(x)} f(x,t)\,\mathrm dt
= \int_{a(x)}^{b(x)} \frac{\partial}{\partial x}f(x,t)\,\mathrm dt+g(x)$\\
$g(x) = f(x,b(x))b'(x) - f(x,a(x))a'(x)$

$\ds \int_{\varphi(U)} f(\underline x)\mathrm d\underline x
= \int_U f(\varphi(\underline u))|\det D\varphi(\underline u)|
\mathrm d\underline u$\\

$T(x) = f(x_0)+f'(x_0)(x-x_0)$\\
$\ds N(x) = f(x_0)-\frac{1}{f'(x_0)}(x-x_0)$

$(n+1)! = (n+1)n!$\\
$\ds\binom{n}{k} = \frac{n!}{k!\,(n-k)!}$\\
$n! = \Gamma(n+1)$\\
$\Gamma(x+1) = x\Gamma(x)$\\
$\ds\Gamma(x)\Gamma(1-x) = \frac{\pi}{\sin(\pi x)}$

${}\!\!\!\begin{array}{l|l}
x = r\cos\varphi & r=\sqrt{x^2+y^2}\\
y = r\sin\varphi & \varphi = \mathrm{sgn}(y)\arccos(x/r)
\end{array}$

$\det J = r$\quad(polar, Zylinder)\\
$\det J = r^2\sin\theta$\quad(Kugel)

$\mathrm{grad}(fg) = g\,\mathrm{grad}\,f+f\,\mathrm{grad}\,g$\\
$\mathrm{div}(fv)
= v\,\mathrm{grad}\,f + f\,\mathrm{grad}\,v$\\
$\mathrm{rot}(fv)
= f\,\mathrm{rot}\,v - v\times\mathrm{grad}\,f$\\
$\mathrm{rot}\,\mathrm{rot}\,v
= \mathrm{grad}\,\mathrm{div}\,v-\Delta v$\\
$\mathrm{div}(v\times w)
= w\,\mathrm{rot}\,v - v\,\mathrm{rot}\,w$\\
$\mathrm{rot}\,\mathrm{grad}\,f=0$\\
$\mathrm{div}\,\mathrm{rot}\,v = 0$

$\ds\begin{bmatrix}
a & b\\
c & d
\end{bmatrix}^{-1}
= \frac{1}{ad-bc}
\begin{bmatrix}
d & -b\\
-c & a
\end{bmatrix}$\\
$\ds R(\varphi) = \begin{bmatrix}
\cos\varphi & -\sin\varphi\\
\sin\varphi & \cos\varphi
\end{bmatrix}$\\
$\begin{bmatrix} a_1\\ a_2\\ a_3
\end{bmatrix}\times
\begin{bmatrix} b_1\\ b_2\\ b_3
\end{bmatrix}
= \begin{bmatrix}
a_2 b_3 - a_3 b_2\\
a_3 b_1 - a_1 b_3\\
a_1 b_2 - a_2 b_1
\end{bmatrix}$

$\ds L\{f(t)\} = \int_0^{\infty} f(t)e^{-pt}\mathrm dt$\\
$\ds F\{f(t)\} = \frac{1}{\sqrt{2\pi}}\int_{-\infty}^{\infty}
f(t)e^{-i\omega t}\mathrm dt$\\
$\ds Z\{a_n\} = \sum_{k=0}^\infty a_k z^{-k}$

$\ds y = \overline y + \frac{s_{xy}}{s_x}(x-\overline x)$

$\nabla f(x,y) + \lambda\nabla g(x,y)=0$\\
$I[y]=\ds\int_a^b F(x,y(x),y'(x))\,\mathrm dx$

$\ds \frac{\partial F}{\partial y}
=\frac{\mathrm d}{\mathrm dx} \frac{\partial F}{\partial y'},\quad
\ds \frac{\partial L}{\partial q}
=\frac{\mathrm d}{\mathrm dt} \frac{\partial L}{\partial\dot q},\quad
\ds \frac{\partial\mathcal L}{\partial\varphi}
=\partial_\mu \frac{\partial\mathcal L}{\partial(\partial_\mu\varphi)}$


% == Physik ==
\newpage


\textbf{Mechanik}

${}\!\!\!\begin{array}{l|l}
v = s'(t) & \omega = \varphi'(t)\\
a = v'(t) & \alpha = \omega'(t)\\
F = p'(t) & L = M'(t)\\
p = mv & L = J\omega\\
F = ma & M = J\alpha\\
E_\mathrm{kin} = \frac{1}{2}mv^2
& E_\mathrm{rot} = \frac{1}{2}J\omega^2
\end{array}$

${}\!\!\!\begin{array}{l|l|l}
s=\varphi r& M=rF & E_\mathrm{pot} = mgh\\
v=\omega r & M=r\times F & E_\mathrm{kin}+E_\mathrm{pot} = \mathrm{const.}\\
a=\alpha r& L=r\times p & F = Ds\quad \mathrm{(Feder)}
\end{array}$


%$s=r\varphi,\quad v=r\omega,\quad a=r\alpha$\\
%$M=rF,\quad M = r\times F$\\
%$E_\mathrm{pot} = mgh$\\
% $E_\mathrm{kin}+E_\mathrm{pot} = \mathrm{const.}$\\
% $F = Ds\quad \mathrm{(Feder)}$

\textbf{Gleichstrom}

${}\!\!\!\begin{array}{l|l|l}
U=RI & Q=It & GR=1\\
I=GU & W=P\;\!t\\
P=UI & W=QU\\
\end{array}$

\textbf{Wechselstrom}

${}\!\!\!\begin{array}{l|l|l}
\underline U = \underline Z\underline I
& \underline Z = R+jX
& Z^2 = R^2+X^2\\
\underline I=\underline Y\underline U
& \underline Y = G+jQ
& R = Z\cos\varphi\\
\underline S = \underline U\underline I
& \underline S = P+jB
& X = Z\sin\varphi
\end{array}$

${}\!\!\!\begin{array}{l|l|l}
\underline Z = R & \mathrm{Widerstand}
& \omega = 2\pi f\\
\underline Z = jX_C & \mathrm{Kondensator}
& X_C = -1/(\omega C)\\
\underline Z = jX_L & \mathrm{Spule}
& X_L = \omega L
\end{array}$

${}\!\!\!\begin{array}{l|l}
u_s = \sqrt{2}\,U_\mathrm{eff}
& u = u_s\sin(\omega t+\varphi_0)\\
i_s = \sqrt{2}\,I_\mathrm{eff}
& i = i_s\sin(\omega t+\varphi_0)
\end{array}$

\textbf{allgemeine Gleichungen}

${}\!\!\!\begin{array}{l|l}
u = Ri & p=ui\\
i = Cu'(t)\\
u = Li'(t)
\end{array}$

\textbf{elektrostatisches Feld}

${}\!\!\!\begin{array}{l|l}
\ds F=\frac{1}{4\pi\varepsilon}\frac{Q_1Q_2}{r^2}
&\ds\vec F_1 = \frac{1}{4\pi\varepsilon}
Q_1Q_2\frac{\underline x_1-\underline x_2}
{|\underline x_1-\underline x_2|^3}
\end{array}$

${}\!\!\!\begin{array}{l|l|l}
\vec F = q\underline E & Q=CU
&U = \varphi(B)-\varphi(A)\\
\underline D = \varepsilon \underline E
&\varepsilon = \varepsilon_0\varepsilon_r
& W=QU
\end{array}$\\
$\underline E = -\mathrm{grad}\,\varphi$\\
$\varepsilon_0 E^2 = 2w_e$

\textbf{Plattenkondensator}

${}\!\!\!\begin{array}{l|l}
U=Ed & C=\varepsilon A/d
\end{array}$

\textbf{homogenes Feld in der Spule}

${}\!\!\!\begin{array}{l|l|l}
H\;\!l = NI & B\;\!l = \mu NI & \Theta = NI
\end{array}$

\textbf{magnetostatisches Feld}

${}\!\!\!\begin{array}{l|l}
\vec F = q\underline v\times\underline B
& \Phi = BA\\
F = qvB & \underline B = \mu\underline H\\
F = BIl & \mu = \mu_0\mu_r
\end{array}$

$H = I/(2\pi r)\quad (\text{Feld um einen geraden Leiter})$\\
$B^2 = 2\mu_0 w_m$

\textbf{Elektrodynamik}

$E=-\nabla\varphi$\\
$\varepsilon\Delta\varphi = -\rho(x)$\\
$\varepsilon_0 E^2 = 2w_e$\\
$B^2 = 2\mu_0 w_m$

\newpage
\textbf{Maxwell-Gleichungen}

${}\!\!\!\begin{array}{l|l}
\langle\nabla,D\rangle = \rho_f(x)
& \langle\nabla,\varepsilon_0 E\rangle = \rho(x)
\\
\langle\nabla,B\rangle = 0
& \langle\nabla,B\rangle = 0\\
\nabla\times E = -D_t B
& \nabla\times E = -D_t B\\
\nabla\times H = J_f+D_t D
& \nabla\times B = \mu_0 (J+\varepsilon_0 D_t E)
\end{array}$


\textbf{SRT}

$\ds \gamma = \frac{1}{\sqrt{1-\beta^2}},\quad\beta=v/c$\\
$\gamma = \cosh\varphi,\quad
\beta\gamma = \sinh\varphi,\quad
\beta = \tanh\varphi$\\
$ct'=\gamma(ct-\beta x),\;\; x'=\gamma(x-vt),
\;\; (y,z)'=(y,z)$\\
${}\!\!\!\begin{array}{l|l}
t=\gamma\tau & E_\mathrm{kin} = E-E_0\\
p=\gamma mv & E_\mathrm{kin} = \gamma mc^2-mc^2\\
E=\gamma mc^2 & E^2 = (pc)^2 + (mc^2)^2\\
\end{array}$\\
$\Lambda_v = \begin{bmatrix}
\gamma & -\beta\gamma & 0 & 0\\
-\beta\gamma & \gamma & 0 & 0\\
0 & 0 & 1 & 0\\
0 & 0 & 0 & 1
\end{bmatrix}$\\
$g=\mathrm{diag}(1,-1,-1,-1)$\\
$(D_\mu) = (D_{ct},D_x,D_y,D_z)$\\
$(D^\mu) = (D_{ct},-D_x,-D_y,-D_z)$

\textbf{Optik}

$\ds\frac{1}{f}=\frac{1}{g}+\frac{1}{b},\quad
A = \frac{B}{G} = \frac{b}{g}$

$n_1\sin(\varphi_1) = n_2\sin(\varphi_2)$\\
$c_0 = nc$

\textbf{Thermodynamik}

${}\!\!\!\begin{array}{l|l|l}
R = N_{\!A} k_B & m = nM & V = nV_m\\
R = R_s M & m = Nm_T & N=nN_{\!A}
\end{array}$

$pV = nRT$\\
$\ds \frac{p_1 V_1}{T_1} = \frac{p_2 V_2}{T_2}$\\
$Q =mc\Delta T$


\textbf{Konstanten}

$\varepsilon_0 = 8.8542\times 10^{-12}\,\mathrm{C/(V\,m)}$\\
$\mu_0 = 4\pi\times 10^{-7}\,\mathrm{H/m}$\\
$c_0 = 2.9979\times 10^{8}\,\mathrm{m/s}$\\
$e = 1.6022\times 10^{-19}\,\mathrm{C}$\\
$G = 6.674\times 10^{-11}\,\mathrm{m^3/(kg\,s^2)}$

$N_{\!A} = 6.0221\times 10^{23}\,\mathrm{mol}^{-1}$\\
$k_B = 1.3806\times 10^{-23}\,\mathrm{J/K}$\\
$R = 8.3145\,\mathrm{J/(mol\,K)}$

$0\,\mathrm K = -273.15\,\mathrm{{}^\circ C}$\\
$u = 1.6605\times 10^{-27}\,\mathrm{kg}$\\
$h = 6.6261\times 10^{-34}\,\mathrm{Js}$\\
$\hbar = 1.0546\times 10^{-34}\,\mathrm{Js}$\\
$\sigma = 5.6704\times 10^{-8}\,\mathrm{W/(m^2 K^4)}$

$m_e = 9.1094\times 10^{-31}\,\mathrm{kg}$\\
$m_p = 1.6726\times 10^{-27}\,\mathrm{kg}$\\
$m_n = 1.6749\times 10^{-27}\,\mathrm{kg}$\\
$m_\alpha = 6.6447\times 10^{-27}\,\mathrm{kg}$

\end{document}






