
\appendix
\chapter{Formelsammlung}

\section{Logik}
\subsection*{Natürliches Schließen}

\noindent
\begin{tabular}{cc@{\qquad}c}
\toprule
& \strong{Einführung} & \strong{Beseitigung}\\[2pt]
\toprule
$\land$
& $\dfrac{\Gamma\vdash A\qquad\Gamma'\vdash B}{\Gamma, \Gamma'\vdash A\land B}$
& $\dfrac{\Gamma\vdash A\land B}{\Gamma\vdash A}\quad\dfrac{\Gamma\vdash A\land B}{\Gamma\vdash B}$\\[14pt]
$\lor$
& $\dfrac{\Gamma\vdash A}{\Gamma\vdash A\lor B}\quad\dfrac{\Gamma\vdash B}{\Gamma\vdash A\lor B}$
& $\dfrac{\Gamma\vdash A\lor B\qquad\Gamma',A\vdash C\qquad\Gamma'',B\vdash C}{\Gamma,\Gamma',\Gamma''\vdash C}$\\[14pt]
$\cond$
& $\dfrac{\Gamma,A\vdash B}{\Gamma\vdash A\Rightarrow B}$
& $\dfrac{\Gamma\vdash A\Rightarrow B\qquad\Gamma'\vdash A}{\Gamma,\Gamma'\vdash B}$\\[14pt]
$\lnot$
& $\dfrac{\Gamma,A\vdash\bot}{\Gamma\vdash\neg A}$
& $\dfrac{\Gamma\vdash \neg A\qquad\Gamma'\vdash A}{\Gamma,\Gamma'\vdash\bot}$\\[14pt]
$\bicond$
& $\dfrac{\Gamma\vdash A\Rightarrow B\qquad\Gamma'\vdash B\Rightarrow A}{\Gamma,\Gamma'\vdash A\Leftrightarrow B}$
& $\dfrac{\Gamma\vdash A\Leftrightarrow B}{\Gamma\vdash A\Rightarrow B}\quad
   \dfrac{\Gamma\vdash A\Leftrightarrow B}{\Gamma\vdash B\Rightarrow A}$\\[14pt]
$\forall$
& $\dfrac{\Gamma\vdash A}{\Gamma\vdash\forall x\colon A}(x\notin\mathrm{FV}(\Gamma))$
& $\dfrac{\Gamma\vdash\forall x\colon A}{\Gamma\vdash A[x:=t]}$\\[14pt]
$\exists$
& $\dfrac{\Gamma\vdash A[x:=t]}{\Gamma\vdash\exists x\colon A}$
& $\!\!\!\!\dfrac{\Gamma\vdash\exists x\colon A\qquad\Gamma', A\vdash B}{\Gamma,\Gamma'\vdash B}
(x\notin\mathrm{FV}(\Gamma,\Gamma',B))\!\!$\\[8pt]
\bottomrule
\end{tabular}\\[8pt]
\begin{small}
\begin{tabular}{cc@{\quad\;\;}c@{\quad\;\;}cc}
\toprule
\strong{Name} & \strong{Kürzel} & \strong{Regel} & \strong{Schema} & \strong{Logik}\\
\midrule[\heavyrulewidth]
Ex falso quodlibet
& EFQ
& $\dfrac{\Gamma\vdash\bot}{\Gamma\vdash A}$
& $\bot\cond A$
& intuitionistisch\\[14pt]
\begin{tabular}{@{}c@{}}Satz vom ausgeschlos-\\ senen Dritten\end{tabular}
& LEM
& $\dfrac{}{\vdash A\lor\lnot A}$
& $A\lor\lnot A$
& klassisch\\[14pt]
\begin{tabular}{@{}c@{}}Beseitigung der\\ Doppelnegation\end{tabular}
& DNE
& $\dfrac{\Gamma\vdash\lnot\lnot A}{\Gamma\vdash A}$
& $\lnot\lnot A\cond A$
& klassisch\\
\bottomrule
\end{tabular}
\end{small}

\newpage
\subsection*{Zulässige Regeln der klassischen Logik}

\begin{small}
\begin{tabular}{c@{\quad\;\;}c@{\quad\;\;}c}
\toprule
\strong{Name} & \strong{Regel} & \strong{Schema}\\
\midrule[\heavyrulewidth]
Modus ponens
& $\dfrac{\Gamma\vdash A\cond B\qquad\Gamma'\vdash A}{\Gamma,\Gamma'\vdash B}$
& $(A\cond B)\land A\cond B$\\[14pt]
Schnittregel
& $\dfrac{\Gamma,A\vdash B\qquad\Gamma'\vdash A}{\Gamma,\Gamma'\vdash B}$
& $(A\cond B)\land A\cond B$\\[14pt]
Kettenschluss
& $\dfrac{\Gamma\vdash A\cond B\qquad\Gamma'\vdash B\cond C}{\Gamma,\Gamma'\vdash A\cond C}$
& $(A\cond B)\land (B\cond C)\cond (A\cond C)$\\[14pt]
Modus tollens
& $\dfrac{\Gamma\vdash A\cond B\qquad\Gamma'\vdash\lnot B}{\Gamma,\Gamma'\vdash\lnot A}$
& $(A\cond B)\land\lnot B\cond\lnot A$\\[14pt]
Kontraposition
& $\dfrac{\Gamma\vdash A\cond B}{\Gamma\vdash \lnot B\cond\lnot A}$
& $(A\cond B)\cond (\lnot B\cond\lnot A)$\\[14pt]
\begin{tabular}{@{}c@{}}umgekehrte\\ Kontraposition\end{tabular}
& $\dfrac{\Gamma\vdash \lnot B\cond\lnot A}{\Gamma\vdash A\cond B}$
& $(\lnot B\cond\lnot A)\cond (A\cond B)$\\[14pt]
\begin{tabular}{@{}c@{}} Modus tollendo\\ ponens\end{tabular}
& $\dfrac{\Gamma\vdash A\lor B\qquad\Gamma'\vdash\lnot A}{\Gamma,\Gamma'\vdash B}$
& $(A\lor B)\land\lnot A\cond B$\\[14pt]
\begin{tabular}{@{}c@{}} Modus ponendo\\ tollens\end{tabular}
& $\dfrac{\Gamma\vdash \lnot(A\land B)\qquad\Gamma'\vdash A}{\Gamma,\Gamma'\vdash\lnot B}$
& $\lnot (A\land B)\land A\cond \lnot B$\\[14pt]
Resolution
& $\dfrac{\Gamma\vdash A\lor B\qquad\Gamma'\vdash\lnot A\lor C}{\Gamma,\Gamma'\vdash B\lor C}$
& $(A\lor B)\land (\lnot A\lor C)\cond B\lor C$\\[14pt]
Exportation
& $\dfrac{\Gamma\vdash A\land B\cond C}{\Gamma\vdash A\cond (B\cond C)}$
& $(A\land B\cond C)\bicond (A\cond (B\cond C))$\\[14pt]
Absorption
& $\dfrac{\Gamma\vdash A\cond B}{\Gamma\vdash A\cond A\land B}$
& $(A\cond B)\bicond (A\cond A\land B)$\\[14pt]
Ersetzungsregel
& $\dfrac{\Gamma\vdash A\bicond B\qquad\Gamma'\vdash C(A)}{\Gamma,\Gamma'\vdash C(B)}$
& $(A\bicond B)\land C(A)\cond C(B)$\\[14pt]
\begin{tabular}{@{}c@{}}Reductio ad\\ absurdum\end{tabular}
& $\dfrac{\Gamma,\lnot A\vdash\lnot B\qquad\Gamma',\lnot A\vdash B}{\Gamma,\Gamma'\vdash A}$
& $(\lnot A\cond B)\land(\lnot A\cond\lnot B)\cond A$\\
\bottomrule
\end{tabular}
\end{small}
